1) renamed Llvmcaml.ml to be llvmcaml.ml to work around a bug of CaIDE, which cannot find source files with capitalized names in its debugger. 2) added the debug script, ocamldb, which is loaded via "source ocamldb" in ocamldebug 3) renamed translator.ml to be llvm2coq.ml, added coq2llvm.ml that translates some Coq data types (typ, constant, bop, cond, data layout) to be llvm AST. 4) when returning variable names from Coq, removed the prefix @ and %, this is consistent with how LLVM works, otherwise we cannot find variables wrt names with prefix @ or %. 5) extracted some functions (getTypeAllocSize) in targetdata.v to be C++ functions in LLVM, otherwise computations over Z or Pos quickly consume all stacks.
git-svn-id: https://webdav.seas.upenn.edu/svn/sol/vol@2694 eef5ea85-cc2e-0410-bd84-0fae1f012da8

src/Parser/coq2llvm.ml
@@ -1,0 +1,188 @@
+open Printf
+open Llvm
+open Llvm_aux
+open Ssa_def
+open Ssa_lib
+
+(** Coq Pretty Printer *)
+let rec translate_typ (ctx:llcontext) (ty:LLVMsyntax.typ) : lltype =
+  match ty with
+  | LLVMsyntax.Coq_typ_int sz -> integer_type ctx sz
+	| LLVMsyntax.Coq_typ_float -> float_type ctx
+	| LLVMsyntax.Coq_typ_double -> double_type ctx
+	| LLVMsyntax.Coq_typ_void -> void_type ctx
+	| LLVMsyntax.Coq_typ_label -> label_type ctx
+	| LLVMsyntax.Coq_typ_metadata -> failwith "Metadata: Not_Supported."
+	| LLVMsyntax.Coq_typ_array (sz, t) -> array_type (translate_typ ctx t) sz
+  | LLVMsyntax.Coq_typ_function (t, ts) -> function_type (translate_typ ctx t) 
+	                                           (Array.of_list (LLVMsyntax.map_list_typ (translate_typ ctx) ts))	
+  | LLVMsyntax.Coq_typ_struct ts -> struct_type ctx 
+	                                    (Array.of_list (LLVMsyntax.map_list_typ (translate_typ ctx) ts))
+  | LLVMsyntax.Coq_typ_pointer t -> pointer_type (translate_typ ctx t)
+
+let rec translate_constant (ctx:llcontext) (c:LLVMsyntax.const) : llvalue = 
+	match c with
+	| LLVMsyntax.Coq_const_int (sz, i) -> const_int (integer_type ctx sz) sz
+	| LLVMsyntax.Coq_const_undef t -> undef (translate_typ ctx t)
+	| LLVMsyntax.Coq_const_null t ->  const_null (translate_typ ctx t)
+	| LLVMsyntax.Coq_const_arr cs -> failwith "const_arr: Not_Supported."
+	| LLVMsyntax.Coq_const_struct cs -> const_struct ctx (Array.of_list (LLVMsyntax.map_list_const (translate_constant ctx) cs))
+  | LLVMsyntax.Coq_const_gid (_,id) -> failwith "const_gid: Not_Supported."
+	
+let translate_value v =
+	match v with
+	| LLVMsyntax.Coq_value_id id ->  failwith "Not_Supported."
+	| LLVMsyntax.Coq_value_const c ->  failwith "Not_Supported."
+
+let rec translate_params ps =
+	match ps with
+	| [] -> ""
+	| (t, v)::ps' -> failwith "Not_Supported."
+
+let rec translate_list_value vs =
+	match vs with
+	| LLVMsyntax.Nil_list_value -> failwith "Not_Supported."
+	| LLVMsyntax.Cons_list_value (v, vs') -> failwith "Not_Supported."
+
+let translate_bop bop =
+	match bop with
+	| LLVMsyntax.Coq_bop_add -> InstrOpcode.Add			
+	| LLVMsyntax.Coq_bop_and -> InstrOpcode.And
+	| LLVMsyntax.Coq_bop_or -> InstrOpcode.Or
+	| LLVMsyntax.Coq_bop_lshr -> InstrOpcode.LShr
+									
+let translate_extop extop =
+	match extop with
+	| LLVMsyntax.Coq_extop_s -> failwith "Not_Supported." 			
+	| LLVMsyntax.Coq_extop_z -> failwith "Not_Supported."
+
+let translate_castop castop =
+	match castop with
+	| LLVMsyntax.Coq_castop_fptoui -> failwith "Not_Supported." 			
+	| LLVMsyntax.Coq_castop_fptosi -> failwith "Not_Supported."	 
+	| LLVMsyntax.Coq_castop_uitofp -> failwith "Not_Supported."
+	| LLVMsyntax.Coq_castop_sitofp -> failwith "Not_Supported."
+  | LLVMsyntax.Coq_castop_ptrtoint -> failwith "Not_Supported."
+	| LLVMsyntax.Coq_castop_inttoptr -> failwith "Not_Supported."
+	| LLVMsyntax.Coq_castop_bitcast -> failwith "Not_Supported."
+
+let translate_icond cond =
+	match cond with
+	| LLVMsyntax.Coq_cond_eq -> Icmp.Eq		
+	| LLVMsyntax.Coq_cond_ne -> Icmp.Ne 			
+	| LLVMsyntax.Coq_cond_ugt -> Icmp.Ugt		
+	| LLVMsyntax.Coq_cond_uge -> Icmp.Uge	
+	| LLVMsyntax.Coq_cond_ult -> Icmp.Ult	
+	| LLVMsyntax.Coq_cond_ule -> Icmp.Ule	
+	| LLVMsyntax.Coq_cond_sgt -> Icmp.Sgt	
+	| LLVMsyntax.Coq_cond_sge -> Icmp.Sge	
+	| LLVMsyntax.Coq_cond_slt -> Icmp.Slt	
+	| LLVMsyntax.Coq_cond_sle -> Icmp.Sle	
+
+let translate_fcond cond =
+	match cond with
+	| LLVMsyntax.Coq_cond_eq -> Fcmp.Oeq		
+	| LLVMsyntax.Coq_cond_ne -> Fcmp.One			
+	| LLVMsyntax.Coq_cond_ugt -> Fcmp.Ugt		
+	| LLVMsyntax.Coq_cond_uge -> Fcmp.Uge	
+	| LLVMsyntax.Coq_cond_ult -> Fcmp.Ult	
+	| LLVMsyntax.Coq_cond_ule -> Fcmp.Ule	
+	| LLVMsyntax.Coq_cond_sgt -> Fcmp.Ogt
+	| LLVMsyntax.Coq_cond_sge -> Fcmp.Oge	
+	| LLVMsyntax.Coq_cond_slt -> Fcmp.Olt	
+	| LLVMsyntax.Coq_cond_sle -> Fcmp.Ole	
+
+let rec translate_list_value_l vls =
+	match vls with
+  | LLVMsyntax.Cons_list_value_l (v, l, vls') ->  failwith "Not_Supported."
+	| LLVMsyntax.Nil_list_value_l -> failwith "Not_Supported."
+
+let rec translate_args args =
+	match args with
+	| [] -> ""
+	| (t, id)::args' -> failwith "Not_Supported."
+
+let translate_terminator i =
+	match i with 
+	| LLVMsyntax.Coq_insn_br (id, v, l1, l2) -> failwith "Not_Supported."
+	| LLVMsyntax.Coq_insn_br_uncond (id, l) -> failwith "Not_Supported."
+  | LLVMsyntax.Coq_insn_return (id, t, v) -> failwith "Not_Supported."
+  | LLVMsyntax.Coq_insn_return_void id -> failwith "Not_Supported."
+  | LLVMsyntax.Coq_insn_unreachable id -> failwith "Not_Supported."
+
+let translate_cmd i =
+	match i with
+  | LLVMsyntax.Coq_insn_bop (id, bop, sz, v1, v2) -> failwith "Not_Supported."
+  | LLVMsyntax.Coq_insn_extractvalue (id, t, v, cs) -> failwith "Not_Supported."
+  | LLVMsyntax.Coq_insn_insertvalue (id, t1, v1, t2, v2, cs) -> failwith "Not_Supported."
+  | LLVMsyntax.Coq_insn_malloc (id, t, sz, align) -> failwith "Not_Supported."
+  | LLVMsyntax.Coq_insn_alloca (id, t, sz, align) -> failwith "Not_Supported."
+  | LLVMsyntax.Coq_insn_free (id, t, v) -> failwith "Not_Supported."
+  | LLVMsyntax.Coq_insn_load (id, t, v, a) -> failwith "Not_Supported."
+  | LLVMsyntax.Coq_insn_store (id, t, v1, v2, a) -> failwith "Not_Supported."
+  | LLVMsyntax.Coq_insn_gep (id, inbounds, t, v, vs) -> failwith "Not_Supported."
+  | LLVMsyntax.Coq_insn_ext (id, extop, t1, v, t2) -> failwith "Not_Supported."
+  | LLVMsyntax.Coq_insn_cast (id, castop, t1, v, t2) -> failwith "Not_Supported."
+  | LLVMsyntax.Coq_insn_icmp (id, cond, t, v1, v2) -> failwith "Not_Supported."
+  | LLVMsyntax.Coq_insn_select (id, v, t, v1, v2) -> failwith "Not_Supported."
+  | LLVMsyntax.Coq_insn_call (id, noret, tailc, t, fid, ps) -> failwith "Not_Supported."
+					
+let translate_phi i =
+	match i with
+	| LLVMsyntax.Coq_insn_phi (id, t, list_v_l) -> failwith "Not_Supported."
+	
+let translate_block b =
+	match b with
+	| LLVMsyntax.Coq_block_intro (l, ps, cs, tmn) -> failwith "Not_Supported."
+
+let translate_fdec f =
+	match f with
+	| LLVMsyntax.Coq_fheader_intro (t, fid, args) -> failwith "Not_Supported."
+
+let translate_fdef f =
+	match f with
+	| LLVMsyntax.Coq_fdef_intro (LLVMsyntax.Coq_fheader_intro (t, fid, args), bs) ->
+    failwith "Not_Supported."
+					  	
+let translate_product g =
+	match g with
+	| LLVMsyntax.Coq_product_gvar (LLVMsyntax.Coq_gvar_intro (id, t, c, a)) -> failwith "Not_Supported." 
+	| LLVMsyntax.Coq_product_fdec f -> failwith "Not_Supported."
+	| LLVMsyntax.Coq_product_fdef f -> failwith "Not_Supported." 
+	
+let translate_layout dlt =
+	match dlt with
+	| LLVMsyntax.Coq_layout_be -> "E-"
+	| LLVMsyntax.Coq_layout_le -> "e-"
+	| LLVMsyntax.Coq_layout_ptr (sz, a1, a2) -> "p:" ^ (string_of_int sz) ^ 
+	                                             ":" ^ (string_of_int a1) ^                   
+																							 ":" ^ (string_of_int a2) ^
+																							 "-"
+	| LLVMsyntax.Coq_layout_int (sz, a1, a2) -> "i:" ^ (string_of_int sz) ^ 
+	                                             ":" ^ (string_of_int a1) ^                   
+																							 ":" ^ (string_of_int a2) ^
+																							 "-"	
+	| LLVMsyntax.Coq_layout_aggr (sz, a1, a2) -> "a:" ^ (string_of_int sz) ^ 
+	                                              ":" ^ (string_of_int a1) ^                   
+																							  ":" ^ (string_of_int a2) ^
+																							  "-"
+	| LLVMsyntax.Coq_layout_stack (sz, a1, a2) -> "s:" ^ (string_of_int sz) ^ 
+	                                               ":" ^ (string_of_int a1) ^                   
+																							   ":" ^ (string_of_int a2) ^
+																							   "-"
+
+let rec _translate_layouts dlts =
+	match dlts with
+  | [] -> ""
+  | dlt::dlts' -> translate_layout dlt ^ _translate_layouts dlts'
+
+let translate_layouts dlts =
+	let td = _translate_layouts dlts in
+	let len = String.length td in
+	if len = 0 then td else String.sub td 0 (len - 1)
+
+let translate_module m =
+	prerr_endline "Translate module (Coq2LLVM):";
+	match m with
+	| LLVMsyntax.Coq_module_intro (dlts, ps) -> ()
+	
