src/Parser/main.ml
@@ -10,7 +10,7 @@ let main in_filename out_filename =
 	
 	dump_module im;
 	Llvm_pretty_printer.travel_module ist im;
-	let coqim = Translator.translate_module ist im in
+	let coqim = Llvm2coq.translate_module ist im in
 	Coq_pretty_printer.travel_module coqim;
 
 	let oc = create_context () in
@@ -18,9 +18,11 @@ let main in_filename out_filename =
 	let om = Llvm_bitreader.parse_bitcode oc ombuf in
 	let ost = SlotTracker.create_of_module om in
 
-	let coqom = Translator.translate_module ost om in
+	let coqom = Llvm2coq.translate_module ost om in
 			
 	eprintf "TV=%b\n" (tv_module coqim coqom);
+	
+	Coq2llvm.translate_module coqom;
 	
 	(* write the module to a file *)
 	(* if not (Llvm_bitwriter.write_bitcode_file m out_filename) then exit 1; *)
